\documentclass[12pt]{article}
\usepackage{../../template}
\title{Lecture 26}
\author{niceguy}
\begin{document}
\maketitle

\section{Plane Wave Incidence on Material Boundaries}

For simple media, the wavenumber is in general

$$k = \omega\sqrt{\varepsilon\mu} = \omega\sqrt{\varepsilon_0\varepsilon_r\mu_0\mu_r} = \omega\sqrt{\varepsilon_0\mu_0}\sqrt{\varepsilon_r\mu_r} = k_0n$$
where we define the \textbf{refractive index} to be
$$n = \sqrt{\varepsilon_r\mu_r}$$

If the incident waves are
\begin{align*}
    \tilde{\vec{E_i}} &= E_ie^{-jk_0n_1z} \hat x \\
    \tilde{\vec{H_i}} &= \frac{E_i}{\eta_1} e^{-jk_0n_1z} \hat y
\end{align*}

The reflected wave will be

\begin{align*}
    \tilde{\vec{E_r}} &= \Gamma E_i e^{jk_0n_1z} \hat x \\
    \tilde{\vec{H_r}} &= -\Gamma \frac{E_i}{\eta_1} e^{jk_0n_1z} \hat y
\end{align*}

where $\Gamma$ is the reflection coefficient. The transmitted wave is
\begin{align*}
    \tilde{\vec{E_t}} &= \tau E_i e^{-jk_0n_2z} \hat x \\
    \tilde{\vec{H_t}} &= \tau \frac{E_i}{\eta_2} e^{-jk_0n_2z} \hat y
\end{align*}

By continuity of tangential $\vec E$ at $z = 0$, we have
\begin{align*}
    \vec E_r + \vec E_i &= \vec E_t \\
    \Gamma E_i \hat x + E_i \hat x &= \tau E_i \hat x \\
    1 + \Gamma &= \tau
\end{align*}

If there is no surface current, the same applies to $\vec H$, so
\begin{align*}
    \frac{E_i}{\eta_1} - \Gamma \frac{E_i}{\eta_1} &= \tau \frac{E_i}{\eta_2} \\
    \frac{1 - \Gamma}{\eta_1} &= \frac{\tau}{\eta_2}
\end{align*}

Solving,
$$\Gamma = \frac{\eta_2-\eta_1}{\eta_2+\eta_1}, \tau = \frac{2\eta_2}{\eta_1 + \eta_2}$$

In a perfect conductor, $\Gamma = -1, \tau = 0$. In the first medium,

\begin{align*}
    \tilde{\vec E}(z < 0) &= E_ie^{-jk_0n_1z} - E_ie^{jk_0n_1z} \hat x \\
                          &= -2jE_0\sin(k_0n_1z) \hat x
\end{align*}

and similarly

$$\tilde{\vec H}(z < 0) = \frac{E_i}{\eta_1} e^{-jk_0n_1z} + \frac{E_i}{\eta_1} e^{jk_0n_1z} = \frac{2E_i}{\eta_1}\cos(k_0n_1z) \hat y$$
At $z = 0$,
\begin{align*}
    \hat n \times (\vec H_2 - \vec H_1) &= \vec J_s \\
    \hat z \times \left(0 - \frac{2E_i}{\eta_1} \hat y\right) &= \vec J_s \\
    \vec J_s &= \frac{2E_i}{\eta_1} \hat x
\end{align*}

\end{document}
