\documentclass[12pt]{article}
\usepackage{../../template}
\title{Lecture 32}
\author{niceguy}
\begin{document}
\maketitle

\section{Parallel Plate Waveguide}

Consider a waveguide composed of parallel plates $x = 0$ and $x = a$. The wave propogates in the $z$ direction.

\subsection{TE mode}

\begin{align*}
    \tilde H_y &= H_0\cos\left(\frac{n\pi x}{a}\right)e^{-j\beta_nz} \\
    \tilde E_x &= \frac{\beta_n}{\omega\varepsilon} H_0\cos\left(\frac{n\pi x}{a}\right) e^{-j\beta_nz} \\
    \tilde E_z &= \frac{j}{\omega\varepsilon} \frac{n\pi}{a} H_0\sin\left(\frac{n\pi x}{a}\right)e^{-j\beta_nz}
\end{align*}

$\beta_n$ is the propagation constant equal to $k\sqrt{1 - \left(\frac{f_{c,n}}{f}\right)^2}$. The cutoff frequency is

$$f_{c,n} = \frac{n}{2\sqrt{\varepsilon\mu}a}$$

Splitting the cosine term in $\tilde H_y$,
$$\tilde H_y = \frac{H_0}{2}\left(e^{j\frac{n\pi}{a}x}e^{-j\beta_nz} + e^{-j\frac{n\pi}{a}x}e^{-j\beta_nz}\right)$$

This can be split into an incident and reflected wave $\vec k = \pm \frac{n\pi}{a}\hat x + \beta_n\hat z$.

\subsection{$\vec k_i$ as a a function of frequency}

$f < f_{c,n} \Rightarrow \beta_n = -ja_n$ and we call this \textit{evanescent}. Else, $\beta_n = k\sqrt{1 - \left(\frac{f_{c,n}}{f}\right)^2}$. Replacing $f$ with $\omega$ and substituting $k = \omega\sqrt{\varepsilon\mu}$, we get
$$\beta_n = \sqrt{\varepsilon\mu}\sqrt{\omega^2-\omega_{c,n}^2}$$

\subsection{TE mode}

\begin{align*}
    \tilde E_y &= E_0\sin\left(\frac{n\pi x}{a}\right)e^{-j\beta_nz} \\
    \tilde H_x &= -\frac{\beta_n}{\omega\mu} E_0\sin\left(\frac{n\pi x}{a}\right) e^{-j\beta_nz} \\
    \tilde H_z &= \frac{j}{\omega\mu} \frac{n\pi}{a} E_0\cos\left(\frac{n\pi x}{a}\right)e^{-j\beta_nz}
\end{align*}

Below $f_{c,1}$, there is no TE mode. Then $\beta_0 = \omega\sqrt{\varepsilon\mu}, v = \frac{\omega}{\beta} = \frac{1}{\sqrt{\varepsilon\mu}}$. At any higher modes, $\beta$ is frequency dependent, and so is $v$, and one can show that
$$v_{p,n} = \frac{1}{\sqrt{\varepsilon\mu}} \times \frac{1}{\sqrt{1 - \left(\frac{f_{c,n}}{f}\right)^2}} > \frac{1}{\sqrt{\varepsilon\mu}}$$

\end{document}
