\documentclass[12pt]{article}
\usepackage{../../template}
\title{Lecture 28}
\author{niceguy}
\begin{document}
\maketitle

\section{Plane Wave Incidence}

\subsection{Incident Wave}

$$\tilde{\vec E_i} = (\cos\theta_i\hat x - \sin\theta_i\hat z)e^{-jk_0n_1\sin\theta_ix}e^{-jk_0n_1\cos\theta_iz}$$
$$\tilde{\vec H_1} = \frac{1}{\eta_1}e^{-jk_0n_1\sin\theta_ix}e^{-jk_0n_1\cos\theta_iz}\hat y$$
$$n_1 = \sqrt{\varepsilon_{r_1}\mu_{r_1}}, \eta_1 = \sqrt{\frac{\mu_1}{\varepsilon_1}}$$

\subsection{Reflected Wave}

$$\tilde{\vec E_r} = \Gamma_\parallel (\cos\theta_r\hat x + \sin\theta_r\hat z)e^{-jk_0n_1\sin\theta_rx}e^{jk_0n_1\cos\theta_rz}$$
$$\tilde{\vec H_r} = -\frac{\Gamma_\parallel}{\eta_1}e^{-jk_0n_1\sin\theta_rx}e^{jk_0n_1\sin\theta_rz}\hat y$$

\subsection{Transmitted Wave}

$$\tilde{\vec E_t} = \tau_\parallel(\cos\theta_t\hat x - \sin\theta_t\hat z)e^{-jk_0n_2\sin\theta_t}e^{-jk_0n_2\cos\theta_tz}$$
$$\tilde{\vec H_t} = \frac{\tau_\parallel}{\eta_2}e^{-jk_0n_2\sin\theta_tx}e^{-jk_0n_2\cos\theta_tz}\hat y$$

\subsection{Boundary Conditions}

$$E_{x,i}(z=0) + E_{x,r}(z=0) = E_{x,t}(z=0)$$
$$H_{y,i}(z=0) + H_{y,r}(z=0) = H_{y,t}(z=0)$$

In order to satisfy this $\forall x$, all exponentials have to agree by identity. This gives the law of reflection $\theta_i = \theta_r$, and also Snell's law $n_1\sin\theta_i = n_2\sin\theta_t$. Cancelling out the exponentials, we obtain

$$\cos\theta_i(1 + \Gamma_\parallel) = \tau_\parallel \cos\theta_t$$

For the magnetic field, we similarly have

$$\frac{1}{\eta_1}(1 - \Gamma_\parallel) = \frac{\tau_\parallel}{\eta_2}$$

Solving the pair of equations, we can find

$$\Gamma_\parallel = \frac{\eta_2\cos\theta_t - \eta_1\cos\theta_i}{\eta_2\cos\theta_t + \eta_1\cos\theta_i}$$
$$\tau_\parallel = \frac{2\eta_2\cos\theta_i}{\eta_2\cos\theta_t + \eta_1\cos\theta_i}$$

For normal incidence, $\theta_i = \theta_r = \theta_t = 0$, so $\Gamma_\parallel = \frac{\eta_2 - \eta_1}{\eta_2 + \eta_1}, \tau_\parallel = \frac{2\eta_2}{\eta_1 + \eta_2}$. \\

Note that

$$\eta_1\cos\theta_i = \frac{\tilde E_{x,i}}{\tilde H_{y,i}}$$
and
$$\eta_2\cos\theta_t = \frac{\tilde E_{x,t}}{\tilde H_{y,t}}$$

From Snell's law, $\exists \theta_i = \theta_c$ at which $\sin\theta_t = 1$. Above this angle, the transmitted wave propagagtes along the $x$ direction. Since $\sin^2\theta_t > 1$, we have $\cos\theta_t = \sqrt{1 - \sin^2\theta_t} = \pm j\alpha$ where $\alpha$ is real. It makes no physical sense to have a growing solution, so the only solution is

$$\tilde E_t, \tilde H_t ~ e^{-jk_0n_2(\pm j\alpha)z} = e^{k_0n_2\alpha z}$$

The exponention can be split into propogation and attenuation terms, i.e.
$$e^{-jk_0n_1\sin\theta_ix}e^{-k_0n_2\alpha z}$$

The transmitted wave has no power, so all power is transferred to the reflected wave. We call this \textbf{total internal reflection}.

\end{document}
